# July 27th Lecture
- The Normal Distribution is a result of the summation of random variables
- The **Lognormal Distribution** is a result of the multiplication of random variables
    - $Y = X_1 X_2 ... X_n$
    - $\ln{Y} = \ln{X_1} + \ln{X_2} + ... + \ln{X_n}$
    - The $\ln{X_i}$ terms are random variables, so based on the Central Limit Theorem, $\ln{Y}$ is normally distributed
    - $Y = e^{\ln{Y}}$ is *lognormal*
- Lognormal Distribution CDF:
    - $F_y(Y) = P(Y \leq y)$
    - $F_y(Y) = P(e^{\ln{Y}} \leq y)$
    - $F_y(Y) = P(\ln{Y} \leq \ln{y})$
    - $F_y(Y) = P(\frac{\ln{Y} - \mu_{\ln{Y}}}{\sigma_{\ln{Y}}} \leq \frac{\ln{y} - \mu_{\ln{Y}}}{\sigma_{\ln{Y}}}) = P(U \leq \frac{\ln{y} - \mu_{\ln{Y}}}{\sigma_{\ln{Y}}}) = \Phi(\frac{\ln{y} - \mu_{\ln{Y}}}{\sigma_{\ln{Y}}})$
        - Note that $\mu_{\ln{Y}}$ is the mean of $\ln{Y}$ which is *not* the same as as taking the natural log of the mean of Y ($\ln{\mu_Y}$)
        - The same applies for the standard deviation
- Lognormal Distribution PDF:
    - $f_Y(y) = \frac{1}{\sqrt{2\pi}\sigma_{\ln{Y}}y}e^{-0.5(\frac{\ln{y}-\mu_{\ln{Y}}}{\sigma_{\ln{Y}}})^2}$
        - $f_Y(y) = \frac{d}{dy}\Phi(\frac{\ln{y} - \mu_{\ln{Y}}}{\sigma_{\ln{Y}}})$
        - $f_Y(y) = \frac{d}{du}\Phi(\frac{\ln{y} - \mu_{\ln{Y}}}{\sigma_{\ln{Y}}})\frac{du}{dy}$
            - Chain rule: $u = \ln{y} \rightarrow \frac{du}{dy} = \frac{1}{y}$
        - $f_Y(y) = \frac{1}{\sqrt{2\pi} \sigma_{\ln{Y}}y} \exp({-\frac{1}{2}(\frac{\ln{y} - \mu_{\ln{Y}}}{\sigma_{\ln{Y}}})^2})$
- Median:
    - $0.5 = \Phi(\frac{\ln{y_{0.5}} - \mu_{\ln{Y}}}{\sigma_{\ln{Y}}})$
    - $\Phi^{-1}(0.5) = 0 = \frac{\ln{y_{0.5}} - \mu_{\ln{Y}}}{\sigma_{\ln{Y}}}$
    - $\ln{y_{0.5}} = \mu_{\ln{Y}}$ 
    - $y_{0.5} = e^{\mu_{\ln{Y}}}$
- Moments:
    - $E[Y^m] = \int_0^{\infty} y^m f_Y(y)dy = (e^{\mu_{\ln{Y}}})^m e^{\frac{1}{2}m^2 \sigma^2_{\ln{Y}}}$
    - This means that:
        - $\mu_Y = E[Y] = e^{\mu_{\ln{Y}}}e^{\frac{1}{2} \sigma^2_{\ln{Y}{}}}$
        - $\sigma_Y = \sqrt{E[Y^2] -\mu^2_Y} = \sqrt{e^{2\mu_{\ln{Y}}}e^{2\sigma^2_{\ln{Y}}} - e^{2\mu_{\ln{Y}}}e^{\sigma^2_{\ln{Y}}}} = \mu_Y \sqrt{e^{\sigma^2_{\ln{Y}}} - 1}$
    - Given $\mu_Y$ and $\sigma_Y$, one can solve for $\mu_{\ln{Y}}$ and $\sigma_{\ln{Y}}$ and vice-versa
        - $\mu_{\ln{Y}} = \ln{\mu_Y} - \frac{1}{2}\sigma^2_{\ln{Y}}$
        - $\sigma^2_{\ln{Y}} = \ln(\frac{\sigma_Y^2}{\mu_Y^2} + 1)$